## Pythagorean:  

$sin^2 \theta + cos^2 \theta = 1$

$1 + tan^2 \theta = sec^2 \theta$

$csc^2 \theta = 1 + cot^2 \theta$

## Ratio:

$tan \theta = \frac{sin \theta}{cos \theta}$

$cot \theta = \frac{cos \theta}{sin \theta}$


## Opposite Angles

$sin (-\theta) = -sin(\theta)$

$cos(-\theta) = cos(\theta)$

$tan(-\theta) = -tan(\theta)$

$cot(-\theta) = -cot(\theta)$

$sec(-\theta) = sec(\theta)$

$csc(-\theta) = -csc(\theta)$

## Compementary Angles

$sin(90-\theta) = cos \theta$

$cos(90-\theta) = sin \theta$

$tan(90-\theta) = cot \theta$

$cot(90-\theta) = tan \theta$

$sec(90-\theta) = csc \theta$

## Supplementary Angles

$sin(180-\theta) = sin \theta$

$cos(180-\theta) = -cos \theta$

$csc(180 - \theta) = csc \theta$

$sec(180-\theta) = -sec \theta$

$tan(180-\theta) = -tan \theta$

$cot(180-\theta) = -cot \theta$

## Sum/Diff of Angles

$sin(\alpha + \beta) = sin(\alpha) cos(\beta) + cos(\alpha) sin(\beta)$

$sin(\alpha - \beta) = sin(\alpha) cos(\beta) - cos(\alpha) sin(\beta)$

$cos(\alpha + \beta) = cos(\alpha) cos(\beta) - sin(\alpha) sin(\beta)$

$cos(\alpha - \beta) = cos(\alpha) cos(\beta) + sin(\alpha) sin(\beta)$

$tan(\alpha + \beta) = \frac{tan(\alpha) + tan(\beta)}{1 - tan(\alpha) tan(\beta)}$

$tan(\alpha - \beta) = \frac{tan(\alpha)-tan(\beta)}{1+ tan(\alpha) tan(\beta)}$

## Double Angle

$sin(2\theta) = 2 sin\theta cos\theta$

$cos(2\theta) = cos^2 \theta - sin^2 \theta = 2cos^\theta - 1 = 1 - 2sin^2\theta$

$tan(2\theta) = \frac{2tan\theta}{1-tan^2 \theta}$

## Half Angle

$sin(\theta / 2) = \pm \sqrt{\frac{1-cos\theta}{2}}$

$cos(\theta/2) = \pm \sqrt{\frac{1+cos\theta}{2}}$

$tan(\theta/2) = \pm \sqrt{(1-cos\theta)(1+cos\theta)}$

## Product-Sum

$sin \alpha + sin \beta = 2 sin \frac{\alpha + \beta}{2} cos\frac{\alpha - \beta}{2}$

$sin \alpha - sin \beta = 2 cos \frac{\alpha + \beta}{2} sin \frac{\alpha - \beta}{2}$

$cos \alpha + cos \beta = 2 cos \frac{\alpha + \beta}{2}cos\frac{\alpha - \beta}{2}$

$cos\alpha - cos\beta = -2 sin \frac{\alpha + \beta}{2} sin \frac{\alpha - \beta}{2}$


## Products

$sin \alpha sin \beta = \frac{cos ( \alpha - \beta ) - cos(\alpha + \beta)}{2}$

$sin \alpha cos \beta = \frac{sin(\alpha + \beta) + sin(\alpha - \beta)}{2}$

$cos \alpha cos \beta = \frac{cos(\alpha + \beta)+cos(\alpha - \beta)}{2}$

